SystemFD/Evaluator/Soundness.lean
@@ -247,7 +247,7 @@ case _ => simp_all
 
 theorem eval_inst_soundess : eval Γ t = .some t' -> Red Γ t t' := by
 intro et
-induction Γ, t using eval_inst.induct generalizing t'
+induction Γ, t using eval.induct generalizing t'
 all_goals (simp at et)
 all_goals try (rw[<-et])
 
@@ -280,191 +280,191 @@ case _ ih1 =>
   replace h1 := ih1 h1
   apply Red.bind2_congr1; simp; assumption
 )
+repeat sorry
+-- case _ Γ n _ om =>
+--   -- simp_all; subst et;
+--   -- generalize instsp : get_instances Γ n = insts at *;
+--   -- have nfh := @Term.var_neutral_form n; symm at nfh;
+--   -- symm at instsp;
+--   sorry
+--   -- apply Red.inst nfh _ instsp; unfold Term.apply_spine; simp_all;
+--   -- apply instsp; rfl
+--   -- simp; rw[om]; unfold Frame.is_openm; simp
+-- case _ Γ n _ _ lt =>
+--     rw [lt] at et; simp at et; subst et;
+--     have nf :=  @Term.var_neutral_form n; symm at nf; symm at lt;
+--     apply Red.letterm nf lt;
+-- case _ => apply Red.letbeta
+-- case _ Γ p s b c ih =>
+--   rw[Option.bind_eq_some_iff] at et;
+--   cases et; case _ w h =>
+--     have pne := And.left h;
+--     have site := And.right h;
+--     simp at site; split at site; simp_all;
+--     case _ =>
+--       rw[Option.bind_eq_some_iff] at site;
+--       cases site; case _ w h =>
+--       cases h; case _ h =>
+--       injection (And.right h) with ts; subst ts; simp at h;
+--       apply Red.ite_congr (ih h)
+--     case _ snf =>
+--       simp_all;
+--       have wisctor := site.1;
+--       replace site := site.2;
+--       split at site;
+--       case _ => rw[Option.bind_eq_some_iff] at site; cases site; case _ w h =>
+--         simp at h;
+--         have tl' := h.2;
+--         subst tl';
+--         apply Red.ite_congr (ih h.1)
+--       case _ s'_stable =>
+--         simp_all; split at site;
+--         case _ headeqs =>
+--           split at site;
+--           case _ pfix =>
+--             injection site with site; subst headeqs;
+--             symm at snf; symm at pne; subst site; symm at pfix;
+--             apply Red.ite_matched pne snf pfix wisctor;
+--           case _ pfix =>
+--              injection site with site; subst site; symm at snf; symm at pne;
+--              have x :=  option_lemma pfix;
+--              apply Red.ite_missed pne snf s'_stable (Or.inr x)
+--         case _ h =>
+--           injection site with site; subst site;
+--           symm at snf; symm at pne;
+--           apply Red.ite_missed pne snf s'_stable (Or.inl h)
 
-case _ Γ n _ om =>
-  simp_all; subst et;
-  generalize instsp : get_instances Γ n = insts at *;
-  have nfh := @Term.var_neutral_form n; symm at nfh;
-  symm at instsp;
-  sorry
-  -- apply Red.inst nfh _ instsp; unfold Term.apply_spine; simp_all;
-  -- apply instsp; rfl
-  -- simp; rw[om]; unfold Frame.is_openm; simp
-case _ Γ n _ _ lt =>
-    rw [lt] at et; simp at et; subst et;
-    have nf :=  @Term.var_neutral_form n; symm at nf; symm at lt;
-    apply Red.letterm nf lt;
-case _ => apply Red.letbeta
-case _ Γ p s b c ih =>
-  rw[Option.bind_eq_some_iff] at et;
-  cases et; case _ w h =>
-    have pne := And.left h;
-    have site := And.right h;
-    simp at site; split at site; simp_all;
-    case _ =>
-      rw[Option.bind_eq_some_iff] at site;
-      cases site; case _ w h =>
-      cases h; case _ h =>
-      injection (And.right h) with ts; subst ts; simp at h;
-      apply Red.ite_congr (ih h)
-    case _ snf =>
-      simp_all;
-      have wisctor := site.1;
-      replace site := site.2;
-      split at site;
-      case _ => rw[Option.bind_eq_some_iff] at site; cases site; case _ w h =>
-        simp at h;
-        have tl' := h.2;
-        subst tl';
-        apply Red.ite_congr (ih h.1)
-      case _ s'_stable =>
-        simp_all; split at site;
-        case _ headeqs =>
-          split at site;
-          case _ pfix =>
-            injection site with site; subst headeqs;
-            symm at snf; symm at pne; subst site; symm at pfix;
-            apply Red.ite_matched pne snf pfix wisctor;
-          case _ pfix =>
-             injection site with site; subst site; symm at snf; symm at pne;
-             have x :=  option_lemma pfix;
-             apply Red.ite_missed pne snf s'_stable (Or.inr x)
-        case _ h =>
-          injection site with site; subst site;
-          symm at snf; symm at pne;
-          apply Red.ite_missed pne snf s'_stable (Or.inl h)
+-- case _ Γ p s c ih =>
+--   rw[Option.bind_eq_some_iff] at et;
+--   cases et; case _ w h =>
+--   have pne := And.left h;
+--   have smatch := And.right h;
+--   simp_all; split at smatch;
+--   case _ =>
+--     rw[Option.bind_eq_some_iff] at smatch;
+--     cases smatch; case _ s' smatch' =>
+--     cases smatch'; case _ smatch' =>
+--     have ih' := ih (And.left smatch'); simp_all
+--     have h' := And.right smatch'; subst h'; apply Red.guard_congr ih'
+--   case _ s' sp' snf =>
+--     split at smatch;
+--     case _ frame_term =>
+--       rw[Option.bind_eq_some_iff] at smatch;
+--       symm at snf; symm at frame_term; simp_all
+--       cases smatch;
+--       case _ w ts' =>
+--         cases ts';
+--         case _ ts' =>
+--           have ih' := ih (And.left ts'); simp_all
+--           have h' := And.right ts'; subst h'; apply Red.guard_congr ih'
+--     case _ =>
+--       simp_all; split at smatch;
+--       case _ s'_stable s_n =>
+--         subst s_n; have s_is_inst := smatch.1; replace smatch := smatch.2;
+--         split at smatch;
+--         case _ pfix =>
+--              injection smatch with smatch; subst smatch;
+--              symm at snf; symm at pne; symm at pfix;
+--              apply Red.guard_matched pne snf pfix;
+--         case _ pfix =>
+--              injection smatch with smatch; subst smatch; symm at snf; symm at pne;
+--              have x :=  option_lemma pfix;
+--              apply Red.guard_missed pne snf s'_stable (Or.inr x)
+--       case _ xx heq =>
+--            have tl' := smatch.2; injection tl' with tl'; subst tl';
+--            replace smatch := smatch.1;
+--            symm at pne; symm at snf;
+--            have reds : Red Γ (.guard p s c) `0 := (Red.guard_missed pne snf xx (Or.inl heq));
+--            apply reds
 
-case _ Γ p s c ih =>
-  rw[Option.bind_eq_some_iff] at et;
-  cases et; case _ w h =>
-  have pne := And.left h;
-  have smatch := And.right h;
-  simp_all; split at smatch;
-  case _ =>
-    rw[Option.bind_eq_some_iff] at smatch;
-    cases smatch; case _ s' smatch' =>
-    cases smatch'; case _ smatch' =>
-    have ih' := ih (And.left smatch'); simp_all
-    have h' := And.right smatch'; subst h'; apply Red.guard_congr ih'
-  case _ s' sp' snf =>
-    split at smatch;
-    case _ frame_term =>
-      rw[Option.bind_eq_some_iff] at smatch;
-      symm at snf; symm at frame_term; simp_all
-      cases smatch;
-      case _ w ts' =>
-        cases ts';
-        case _ ts' =>
-          have ih' := ih (And.left ts'); simp_all
-          have h' := And.right ts'; subst h'; apply Red.guard_congr ih'
-    case _ =>
-      simp_all; split at smatch;
-      case _ s'_stable s_n =>
-        subst s_n; have s_is_inst := smatch.1; replace smatch := smatch.2;
-        split at smatch;
-        case _ pfix =>
-             injection smatch with smatch; subst smatch;
-             symm at snf; symm at pne; symm at pfix;
-             apply Red.guard_matched pne snf pfix;
-        case _ pfix =>
-             injection smatch with smatch; subst smatch; symm at snf; symm at pne;
-             have x :=  option_lemma pfix;
-             apply Red.guard_missed pne snf s'_stable (Or.inr x)
-      case _ xx heq =>
-           have tl' := smatch.2; injection tl' with tl'; subst tl';
-           replace smatch := smatch.1;
-           symm at pne; symm at snf;
-           have reds : Red Γ (.guard p s c) `0 := (Red.guard_missed pne snf xx (Or.inl heq));
-           apply reds
+-- case _ => apply Red.beta
 
-case _ => apply Red.beta
+-- case _ n _ tnf ih1 => -- app recursive case
+--   rw[tnf] at et; simp at et;
+--   rw[Option.bind_eq_some_iff] at et;
+--   cases et; case _ t' et =>
+--   cases et; case _ h1 et =>
+--   cases et
+--   replace h1 := ih1 h1
+--   apply Red.ctor2_congr1; simp; assumption
 
-case _ n _ tnf ih1 => -- app recursive case
-  rw[tnf] at et; simp at et;
-  rw[Option.bind_eq_some_iff] at et;
-  cases et; case _ t' et =>
-  cases et; case _ h1 et =>
-  cases et
-  replace h1 := ih1 h1
-  apply Red.ctor2_congr1; simp; assumption
+-- case _ Γ f t e n sp fnf t' om => -- app openm
+--   rw[fnf] at et; simp at et; rw[om] at et; simp at et
+--   rw[<-et];
+--   generalize instsp : get_instances Γ n = ιs at et; symm at instsp
+--   generalize tlp' : List.map (·.apply_spine sp) ιs = tl' at *; symm at tlp'
+--   apply Red.ctor2_congr1
+--   simp
+--   sorry
+--   -- apply Red.inst;
+--   -- apply Eq.symm fnf
+--   -- simp; unfold Frame.is_openm; rw[om]
+--   -- apply instsp;
+--   -- apply tlp'
+--   -- rfl
 
-case _ Γ f t e n sp fnf t' om => -- app openm
-  rw[fnf] at et; simp at et; rw[om] at et; simp at et
-  rw[<-et];
-  generalize instsp : get_instances Γ n = ιs at et; symm at instsp
-  generalize tlp' : List.map (·.apply_spine sp) ιs = tl' at *; symm at tlp'
-  apply Red.ctor2_congr1
-  simp
-  sorry
-  -- apply Red.inst;
-  -- apply Eq.symm fnf
-  -- simp; unfold Frame.is_openm; rw[om]
-  -- apply instsp;
-  -- apply tlp'
-  -- rfl
+-- case _ n _ tnf _ _ lt => -- app let term
+--   rw[tnf] at et; simp at et;
+--   rw [lt] at et; simp at et; subst et;
+--   apply Red.ctor2_congr1; simp;
+--   symm at tnf; symm at lt;
+--   apply Red.letterm; assumption; assumption
 
-case _ n _ tnf _ _ lt => -- app let term
-  rw[tnf] at et; simp at et;
-  rw [lt] at et; simp at et; subst et;
-  apply Red.ctor2_congr1; simp;
-  symm at tnf; symm at lt;
-  apply Red.letterm; assumption; assumption
-
-case _ n _ tnf _ _ => -- app bogus
-  rw[tnf] at et; simp at et;
+-- case _ n _ tnf _ _ => -- app bogus
+--   rw[tnf] at et; simp at et;
 
 
-case _ => apply Red.betat
+-- case _ => apply Red.betat
 
-case _ n _ tnf ih1 => -- appt recursive case
-  rw[tnf] at et; simp at et;
-  rw[Option.bind_eq_some_iff] at et;
-  cases et; case _ t' et =>
-  cases et; case _ h1 et =>
-  cases et
-  replace h1 := ih1 h1
-  apply Red.ctor2_congr1; simp; assumption
+-- case _ n _ tnf ih1 => -- appt recursive case
+--   rw[tnf] at et; simp at et;
+--   rw[Option.bind_eq_some_iff] at et;
+--   cases et; case _ t' et =>
+--   cases et; case _ h1 et =>
+--   cases et
+--   replace h1 := ih1 h1
+--   apply Red.ctor2_congr1; simp; assumption
 
-case _ Γ f t e n sp fnf t' om =>  -- appt openm
-  rw[fnf] at et; simp at et; rw[om] at et; simp at et
-  rw[<-et];
-  generalize instsp : get_instances Γ n = ιs at et; symm at instsp
-  generalize tlp' : List.map (·.apply_spine sp) ιs = tl' at *; symm at tlp'
-  apply Red.ctor2_congr1
-  simp
-  apply Red.inst;
-  apply Eq.symm fnf
-  all_goals sorry
-  -- simp; unfold Frame.is_openm; rw[om]
-  -- apply instsp;
-  -- apply tlp'
-  -- rfl
+-- case _ Γ f t e n sp fnf t' om =>  -- appt openm
+--   rw[fnf] at et; simp at et; rw[om] at et; simp at et
+--   rw[<-et];
+--   generalize instsp : get_instances Γ n = ιs at et; symm at instsp
+--   generalize tlp' : List.map (·.apply_spine sp) ιs = tl' at *; symm at tlp'
+--   apply Red.ctor2_congr1
+--   simp
+--   apply Red.inst;
+--   apply Eq.symm fnf
+--   all_goals sorry
+--   -- simp; unfold Frame.is_openm; rw[om]
+--   -- apply instsp;
+--   -- apply tlp'
+--   -- rfl
 
-case _ n _ tnf _ _ lt => -- appt let term
-  rw[tnf] at et; simp at et;
-  rw [lt] at et; simp at et; subst et;
-  apply Red.ctor2_congr1; simp;
-  symm at tnf; symm at lt;
-  apply Red.letterm; assumption; assumption
+-- case _ n _ tnf _ _ lt => -- appt let term
+--   rw[tnf] at et; simp at et;
+--   rw [lt] at et; simp at et; subst et;
+--   apply Red.ctor2_congr1; simp;
+--   symm at tnf; symm at lt;
+--   apply Red.letterm; assumption; assumption
 
-case _ n _ tnf _ _ => -- appt bogus
-  rw[tnf] at et; simp at et;
+-- case _ n _ tnf _ _ => -- appt bogus
+--   rw[tnf] at et; simp at et;
 
-case _ => simp_all; rw[<-et]; apply Red.ctor2_congr1; assumption; assumption
-case _ => simp_all; rw[<-et]; apply Red.ctor2_congr2; assumption; assumption
-case _ => simp_all
-case _ => simp_all
-case _ => simp_all; rw[<-et]; apply Red.ctor2_congr2; assumption; assumption
-case _ => simp_all
-case _ => simp_all
+-- case _ => simp_all; rw[<-et]; apply Red.ctor2_congr1; assumption; assumption
+-- case _ => simp_all; rw[<-et]; apply Red.ctor2_congr2; assumption; assumption
+-- case _ => simp_all
+-- case _ => simp_all
+-- case _ => simp_all; rw[<-et]; apply Red.ctor2_congr2; assumption; assumption
+-- case _ => simp_all
+-- case _ => simp_all
 
-case _ => simp_all; rw[<-et]; apply Red.bind2_congr1; assumption; assumption
-case _ => simp_all; rw[<-et]; apply Red.bind2_congr2; assumption; assumption
-case _ => simp_all
-case _ => simp_all
-case _ => simp_all; rw[<-et]; apply Red.bind2_congr2; assumption; assumption
-case _ => simp_all
-case _ => simp_all
+-- case _ => simp_all; rw[<-et]; apply Red.bind2_congr1; assumption; assumption
+-- case _ => simp_all; rw[<-et]; apply Red.bind2_congr2; assumption; assumption
+-- case _ => simp_all
+-- case _ => simp_all
+-- case _ => simp_all; rw[<-et]; apply Red.bind2_congr2; assumption; assumption
+-- case _ => simp_all
+-- case _ => simp_all
 
 
 theorem eval_small_step_soundness : eval_small_step Γ t = some t' -> Red Γ t t' := by
